Extract common definitions into files for heuristic/provable parameter sets
Avoid duplication of common aliases for functions and types in the various
individual parameter sets by having a single set of common ones that vary
only between heuristic and provable, and include it in the per-parameter set
definition file.

Change check_ES to be properly polymorphic for the parameter sets, instead
of only suitable to the provable parameter sets.

qtesla/code/params-p-I/Hacl.Impl.QTesla.Params.fst
@@ -18,46 +18,7 @@ module UI64 = FStar.UInt64
 
 #reset-options "--z3rlimit 100 --max_fuel 0 --max_ifuel 0 --admit_smt_queries true"
 
-type elem = I64.t
-unfold let to_elem = I64.int_to_t
-module IElem = FStar.Int64
-unfold let elem_n = IElem.n
-
-unfold let sparse_elem = I8.t
-unfold let to_sparse_elem = I8.int_to_t
-unfold let sparse_to_int16 = int8_to_int16
-
-unfold let elem_to_int8 = int64_to_int8
-unfold let int8_to_elem = int8_to_int64
-unfold let elem_to_uint8 = int64_to_uint8
-unfold let uint8_to_elem = uint8_to_int64
-unfold let elem_to_int16 = int64_to_int16
-unfold let int16_to_elem = int16_to_int64
-unfold let elem_to_int32 = int64_to_int32
-unfold let int32_to_elem = int32_to_int64
-unfold let elem_to_uint32 = int64_to_uint32
-unfold let uint32_to_elem = uint32_to_int64
-unfold let elem_to_int64 x = x
-unfold let int64_to_elem x = x
-unfold let elem_to_uint64 = int64_to_uint64
-unfold let uint64_to_elem = uint64_to_int64
-
-unfold let op_Plus_Hat = IElem.op_Plus_Hat
-unfold let op_Subtraction_Hat = IElem.op_Subtraction_Hat
-unfold let op_Star_Hat = IElem.op_Star_Hat
-unfold let op_Slash_Hat = IElem.op_Slash_Hat
-unfold let op_Percent_Hat = IElem.op_Percent_Hat
-unfold let op_Hat_Hat = IElem.op_Hat_Hat
-unfold let op_Amp_Hat = IElem.op_Amp_Hat
-unfold let op_Bar_Hat = IElem.op_Bar_Hat
-unfold let op_Less_Less_Hat = IElem.op_Less_Less_Hat
-unfold let op_Greater_Greater_Hat = IElem.op_Greater_Greater_Hat
-unfold let op_Equals_Hat = IElem.op_Equals_Hat
-unfold let op_Greater_Hat = IElem.op_Greater_Hat
-unfold let op_Greater_Equals_Hat = IElem.op_Greater_Equals_Hat
-unfold let op_Less_Hat = IElem.op_Less_Hat
-unfold let op_Less_Equals_Hat = IElem.op_Less_Equals_Hat
-unfold let lognot = IElem.lognot
+include Hacl.Impl.QTesla.ProvableParameters
 
 /// Parameters in QTesla.Params aren't marked as unfold or inline_for_extraction;
 /// so we need to normalize them here
