qtesla/code/Hacl.Impl.QTesla.ProvableParameters.fst
@@ -1,0 +1,64 @@
+// Common types and functions for provable parameter sets: p-I and p-III
+module Hacl.Impl.QTesla.ProvableParameters
+
+#reset-options "--z3rlimit 100 --max_fuel 0 --max_ifuel 0 --admit_smt_queries true"
+
+module I8 = FStar.Int8
+module I16 = FStar.Int16
+module I64 = FStar.Int64
+open FStar.Int.Cast
+open Lib.IntTypes
+
+type elem = I64.t
+unfold let to_elem = I64.int_to_t
+module IElem = FStar.Int64
+unfold let elem_n = IElem.n
+
+unfold let elem_to_int8 = int64_to_int8
+unfold let int8_to_elem = int8_to_int64
+unfold let elem_to_uint8 = int64_to_uint8
+unfold let uint8_to_elem = uint8_to_int64
+unfold let elem_to_int16 = int64_to_int16
+unfold let int16_to_elem = int16_to_int64
+unfold let elem_to_int32 = int64_to_int32
+unfold let int32_to_elem = int32_to_int64
+unfold let elem_to_uint32 = int64_to_uint32
+unfold let uint32_to_elem = uint32_to_int64
+unfold let elem_to_int64 x = x
+unfold let int64_to_elem x = x
+unfold let elem_to_uint64 = int64_to_uint64
+unfold let uint64_to_elem = uint64_to_int64
+
+unfold let sparse_elem = I8.t
+unfold let to_sparse_elem = I8.int_to_t
+unfold let sparse_to_int16 = int8_to_int16
+
+unfold let checkES_t = I16.t
+unfold let checkES_n = FStar.UInt32.uint_to_t I16.n
+unfold let checkES_init = 0s
+unfold let elem_to_checkES_t = elem_to_int16
+unfold let checkES_plus = I16.op_Plus_Hat
+unfold let checkES_minus = I16.op_Subtraction_Hat
+unfold let checkES_sr = I16.op_Greater_Greater_Hat
+unfold let checkES_and = I16.op_Amp_Hat
+unfold let checkES_or = I16.op_Bar_Hat
+unfold let checkES_lognot = I16.lognot
+unfold let checkES_to_uint32 = int16_to_uint32
+
+unfold let op_Plus_Hat = IElem.op_Plus_Hat
+unfold let op_Subtraction_Hat = IElem.op_Subtraction_Hat
+unfold let op_Star_Hat = IElem.op_Star_Hat
+unfold let op_Slash_Hat = IElem.op_Slash_Hat
+unfold let op_Percent_Hat = IElem.op_Percent_Hat
+unfold let op_Hat_Hat = IElem.op_Hat_Hat
+unfold let op_Amp_Hat = IElem.op_Amp_Hat
+unfold let op_Bar_Hat = IElem.op_Bar_Hat
+unfold let op_Less_Less_Hat = IElem.op_Less_Less_Hat
+unfold let op_Greater_Greater_Hat = IElem.op_Greater_Greater_Hat
+unfold let op_Equals_Hat = IElem.op_Equals_Hat
+unfold let op_Greater_Hat = IElem.op_Greater_Hat
+unfold let op_Greater_Equals_Hat = IElem.op_Greater_Equals_Hat
+unfold let op_Less_Hat = IElem.op_Less_Hat
+unfold let op_Less_Equals_Hat = IElem.op_Less_Equals_Hat
+unfold let lognot = IElem.lognot
+
